raft/TermsAndIndicesFromOneInterface.v
@@ -14,11 +14,6 @@ Section TermsAndIndicesFromOne.
   Context {one_node_params : OneNodeParams orig_base_params}.
   Context {raft_params : RaftParams orig_base_params}.
 
-  Definition terms_and_indices_from_one (l : list entry) : Prop :=
-    forall e,
-      In e l ->
-      eTerm e >= 1 /\ eIndex e >= 1.
-
   Definition terms_and_indices_from_one_vwl (net : network) : Prop :=
     forall h t h' log,
       In (t, h', log) (votesWithLog (fst (nwState net h))) ->
