raft/proof/TermsAndIndicesFromOneLogProof.v
@@ -1,0 +1,152 @@
+Require Import List.
+Import ListNotations.
+
+Require Import VerdiTactics.
+Require Import Util.
+Require Import Net.
+
+Require Import Raft.
+Require Import RaftRefinementInterface.
+Require Import CommonDefinitions.
+Require Import SpecLemmas.
+
+Require Import UpdateLemmas.
+Local Arguments update {_} {_} {_} _ _ _ _ : simpl never.
+
+Require Import TermsAndIndicesFromOneLogInterface.
+Require Import CurrentTermGtZeroInterface.
+
+Section TermsAndIndicesFromOneLog.
+  Context {orig_base_params : BaseParams}.
+  Context {one_node_params : OneNodeParams orig_base_params}.
+  Context {raft_params : RaftParams orig_base_params}.
+  Context {ctgzi : current_term_gt_zero_interface}.
+
+  Lemma terms_and_indices_from_one_log_init :
+    raft_net_invariant_init terms_and_indices_from_one_log.
+  Proof.
+    unfold raft_net_invariant_init, terms_and_indices_from_one_log.
+    unfold terms_and_indices_from_one. simpl. contradiction.
+  Qed.
+
+  Ltac update_destruct :=
+    match goal with
+      | [ |- context [ update _ ?y _ ?x ] ] => destruct (name_eq_dec y x)
+      | [ H : context [ update _ ?y _ ?x ] |- _ ] => destruct (name_eq_dec y x)
+    end.
+
+  Lemma terms_and_indices_from_one_log_client_request :
+    raft_net_invariant_client_request terms_and_indices_from_one_log.
+  Proof.
+    unfold raft_net_invariant_client_request, terms_and_indices_from_one_log.
+    simpl. intuition. find_higher_order_rewrite. update_destruct; subst; rewrite_update.
+    - find_apply_lem_hyp handleClientRequest_log. intuition.
+      + repeat find_rewrite. auto.
+      + break_exists. intuition. unfold terms_and_indices_from_one in *.
+        intros. repeat find_rewrite. simpl in *. break_or_hyp.
+        * intuition. find_apply_lem_hyp current_term_gt_zero_invariant.
+          find_rewrite. eapply_prop current_term_gt_zero. congruence.
+        * eauto.
+    - auto.
+  Qed.
+
+  Lemma terms_and_indices_from_one_log_timeout :
+    raft_net_invariant_timeout terms_and_indices_from_one_log.
+  Proof.
+    unfold raft_net_invariant_timeout, terms_and_indices_from_one_log.
+    simpl. intuition. find_higher_order_rewrite. update_destruct; subst; rewrite_update; auto.
+    find_apply_lem_hyp handleTimeout_log_same. find_rewrite. auto.
+  Qed.
+
+  Lemma terms_and_indices_from_one_log_append_entries :
+    raft_net_invariant_append_entries terms_and_indices_from_one_log.
+  Proof.
+    unfold raft_net_invariant_append_entries, terms_and_indices_from_one_log.
+    simpl. intuition. find_higher_order_rewrite. update_destruct; subst; rewrite_update; auto.
+    find_apply_lem_hyp handleAppendEntries_log. intuition.
+    - find_rewrite. auto.
+    - subst. unfold terms_and_indices_from_one. admit.
+    - break_exists. intuition. subst. unfold terms_and_indices_from_one in *.
+      intros. find_rewrite. admit.
+  Qed.
+
+  Lemma terms_and_indices_from_one_log_append_entries_reply :
+    raft_net_invariant_append_entries_reply terms_and_indices_from_one_log.
+  Proof.
+    unfold raft_net_invariant_append_entries_reply, terms_and_indices_from_one_log.
+    simpl. intuition. find_higher_order_rewrite. update_destruct; subst; rewrite_update; auto.
+    find_apply_lem_hyp handleAppendEntriesReply_log. find_rewrite. auto.
+  Qed.
+
+  Lemma terms_and_indices_from_one_log_request_vote :
+    raft_net_invariant_request_vote terms_and_indices_from_one_log.
+  Proof.
+    unfold raft_net_invariant_request_vote, terms_and_indices_from_one_log.
+    simpl. intuition. find_higher_order_rewrite. update_destruct; subst; rewrite_update; auto.
+    find_apply_lem_hyp handleRequestVote_log. find_rewrite. auto.
+  Qed.
+
+  Lemma terms_and_indices_from_one_log_request_vote_reply :
+    raft_net_invariant_request_vote_reply terms_and_indices_from_one_log.
+  Proof.
+    unfold raft_net_invariant_request_vote_reply, terms_and_indices_from_one_log.
+    simpl. intuition. find_higher_order_rewrite. update_destruct; rewrite_update; auto.
+    symmetry in H. find_apply_lem_hyp handleRequestVoteReply_log. subst. find_rewrite. auto.
+  Qed.
+
+  Lemma terms_and_indices_from_one_log_do_leader :
+    raft_net_invariant_do_leader terms_and_indices_from_one_log.
+  Proof.
+    unfold raft_net_invariant_do_leader, terms_and_indices_from_one_log.
+    simpl. intuition. find_higher_order_rewrite. update_destruct; subst; rewrite_update; auto.
+    find_apply_lem_hyp doLeader_log. find_rewrite. auto.
+  Qed.
+
+  Lemma terms_and_indices_from_one_log_do_generic_server :
+    raft_net_invariant_do_generic_server terms_and_indices_from_one_log.
+  Proof.
+    unfold raft_net_invariant_do_generic_server, terms_and_indices_from_one_log.
+    simpl. intuition. find_higher_order_rewrite. update_destruct; subst; rewrite_update; auto.
+    find_apply_lem_hyp doGenericServer_log. find_rewrite. auto.
+  Qed.
+
+  Lemma terms_and_indices_from_one_log_state_same_packet_subset :
+    raft_net_invariant_state_same_packet_subset terms_and_indices_from_one_log.
+  Proof.
+    unfold raft_net_invariant_state_same_packet_subset, terms_and_indices_from_one_log.
+    simpl. intuition. find_reverse_higher_order_rewrite. auto.
+  Qed.
+
+  Lemma terms_and_indices_from_one_log_reboot :
+    raft_net_invariant_reboot terms_and_indices_from_one_log.
+  Proof.
+    unfold raft_net_invariant_reboot, terms_and_indices_from_one_log.
+    simpl. intuition. find_higher_order_rewrite. update_destruct; subst; rewrite_update; auto.
+    unfold reboot. simpl. auto.
+  Qed.
+
+  Lemma terms_and_indices_from_one_log_invariant :
+    forall net,
+      raft_intermediate_reachable net ->
+      terms_and_indices_from_one_log net.
+  Proof.
+    intros.
+    apply raft_net_invariant; auto.
+    - apply terms_and_indices_from_one_log_init.
+    - apply terms_and_indices_from_one_log_client_request.
+    - apply terms_and_indices_from_one_log_timeout.
+    - apply terms_and_indices_from_one_log_append_entries.
+    - apply terms_and_indices_from_one_log_append_entries_reply.
+    - apply terms_and_indices_from_one_log_request_vote.
+    - apply terms_and_indices_from_one_log_request_vote_reply.
+    - apply terms_and_indices_from_one_log_do_leader.
+    - apply terms_and_indices_from_one_log_do_generic_server.
+    - apply terms_and_indices_from_one_log_state_same_packet_subset.
+    - apply terms_and_indices_from_one_log_reboot.
+  Qed.
+
+  Instance taifoli : terms_and_indices_from_one_log_interface.
+  Proof.
+    split. apply terms_and_indices_from_one_log_invariant.
+  Qed.
+End TermsAndIndicesFromOneLog.
